add login dafny

system.dfy
@@ -1,73 +1,217 @@
-class {:autocontracts} System
+class {:autocontracts} UserTable
 {
-    ghost var userID: int;
-    ghost var username: string;
-    ghost var businessID: int;
-    ghost var error: int;
+    var id: int;
+    var username: string;
+    var password: string;
+    var first_name: string;
+    var last_name: string
+    var phone_no: string
+    var email: string;
     
-    predicate Valid()
-    {
-    }
-    
-    constructor()
-    {
-    }
-    
-    method Login(username: array<char>, password: array<char>) returns (userID: int)
-    requires username.Length > 0 && password.Length > 0;
-    {
-    }
-    
-    method SignUp()
-    {
-    }
-    
-    method Search()
-    {
-    }
-    
-    method NewRequest()
-    {
-    }
-    
-    method LinkBusiness()
-    {
-    }
-    
-    method EditBusiness()
-    {
-    }
-    
-    method NewBid()
-    {
-    }
-    
-    method EditBid()
-    {
-    }
-    
-    method RemoveBid()
-    {
-    }
-    
-    method DeleteBid()
-    {
-    }
-    
-    method AcceptBid()
-    {
-    }
-    
-    method DeleteRequest()
-    {
-    }
-    
-    method EditRequest()
-    {
-    }
-    
-    method Search()
-    {
-    }
+//    constructor()
+//    {
+//        this.id := 0;
+//        this.username := new string[0];
+//        this.password := new string[0];
+//        this.first_name := new string[0];
+//        this.last_name := new string[0];
+//        this.phone_no := new string[0];
+//        this.email := new string[0];
+//    }
+
+      constructor(user: string, pass: string, first: string, last: string, phone: string, email: string)
+      {
+          this.id := 0;
+          this.username := user;
+          this.password := pass;
+          this.first_name := first;
+          this.last_name := last;
+          this.phone_no := phone;
+          this.email := email;
+      }
+      
+      method setID(id: int)
+      requires id >= 0;
+      { this.id := id; }
 }
 
+class {:autocontracts} System<UserTable(0)>
+{
+    var userID: int;
+    var username: string;
+    var businessID: int;
+    
+    ghost var error: int;
+    
+    var Users: array<UserTable>;
+//    var Requests: array<RequestTable>;
+//    var Businesses: array<BusinessTable>;
+//    var Bids: array<BidTable>;
+//    var RateSum: array<RateSumTable>;
+//    var Ratings: array<RatingTable>;
+    
+    predicate Valid()
+    { -1 <= this.userID < this.Users.Length }
+    
+//    predicate unique_username()
+//    reads this.Users;
+//    reads set m | 0 <= m < this.Users.Length :: this.Users[m];
+//    { forall i, j:: 0 <= i < j < this.Users.Length ==> this.Users[i].username != this.Users[j].username }
+//    
+//    predicate unique_email()
+//    reads this.Users;
+//    reads set m | 0 <= m < this.Users.Length :: this.Users[m];
+//    { forall i, j:: 0 <= i < j < this.Users.Length ==> this.Users[i].email != this.Users[j].email }
+    
+    predicate login_required()
+    { |this.username| > 0 }
+    
+    
+//    predicate bidder_required()
+//    {  }
+    
+//    method Init()
+//    ensures this.userID == -1 && this.username == "" && this.businessID == -1 && this.error == 0;
+//    {
+//        this.userID := -1; // null
+//        this.username := ""; // null
+//        this.businessID := -1; // null
+//        this.error := 0; // no error
+//        
+//        this.Users := new UserTable[0];        
+//    }
+
+    constructor()
+    //requires size >=0;
+    ensures this.userID == -1 && this.username == "" && this.businessID == -1 && this.error == 0;
+    {
+        this.userID := -1; // null
+        this.username := ""; // null
+        this.businessID := -1; // null
+        this.error := 0; // no error
+        
+        this.Users := new UserTable[0];        
+    }
+    
+    method Login(username: string, password: string) returns (userID: int)
+    requires |username| > 0 && |password| > 0;
+    {
+        var i := 0;
+        this.error := 1;
+        while (i < this.Users.Length)
+        invariant 0 <= i <= this.Users.Length;
+        {
+            if (this.Users[i].username == username && this.Users[i].password == password)
+            {
+                this.userID := i;
+                this.username := username;
+                this.error := 0;
+                return i;
+            }
+            i := i + 1;
+        }
+        return -1;
+    }
+    
+    method SignUp(first: string, last: string, username: string, pass: string, repass: string, phone: string, email: string) returns (err: int)
+    ensures err == 0 || err == 1;
+    ensures this.error == 0 ==> err == 0;
+    ensures this.error != 0 ==> err == 1;
+    //ensures forall i:: 0 <= i < old(this.Users.Length) ==> this.Users[i] == old(this.Users[i]);
+    ensures err == 0 ==> this.Users.Length == old(this.Users.Length) + 1 && this.Users[old(this.Users.Length)].username == username &&
+            this.Users[old(this.Users.Length)].password == pass && this.Users[old(this.Users.Length)].email == email;
+    {
+        this.error := 0;
+        err := 0;
+        var i := 0;
+        while (i < this.Users.Length && err == 0)
+        invariant 0 <= i <= this.Users.Length;
+        invariant this.error == 0 ==> err == 0;
+        invariant this.error != 0 ==> err == 1;
+        {
+            if (pass != repass)
+            {
+                this.error := 3;
+                err := 1;
+            }
+            if (this.Users[i].username == username)
+            {
+                this.error := 1;
+                err := 1;
+            }
+            if (this.Users[i].email == email)
+            {
+                this.error := 2;
+                err := 1;
+            }
+            i := i + 1;
+        }
+        if (err == 0)
+        {
+            //add in
+            var newUser := new UserTable(username, pass, first, last, phone, email);
+            newUser.setID(this.Users.Length);
+            //var size := this.Users.Length + 1;
+            var updateUsers: array<UserTable> := new UserTable[this.Users.Length + 1];
+            forall i | 0 <= i < this.Users.Length { updateUsers[i] := this.Users[i]; }
+            updateUsers[this.Users.Length] := newUser;
+            this.Users := updateUsers;
+        }
+        //return err;
+    }
+    
+//    method Search()
+//    {
+//    }
+//    
+//    method NewRequest()
+//    {
+//    }
+//    
+//    method LinkBusiness()
+//    {
+//    }
+//    
+//    method EditBusiness()
+//    {
+//    }
+//    
+//    method NewBid()
+//    {
+//    }
+//    
+//    method EditBid()
+//    {
+//    }
+//    
+//    method RemoveBid()
+//    {
+//    }
+//    
+//    method DeleteBid()
+//    {
+//    }
+//    
+//    method AcceptBid()
+//    {
+//    }
+//    
+//    method DeleteRequest()
+//    {
+//    }
+//    
+//    method EditRequest()
+//    {
+//    }
+//    
+//    method Search()
+//    {
+//    }
+}
+
+method Main()
+{
+    var PartyWhip := new System();
+    //PartyWhip.init();
+    assert PartyWhip.username == "" && PartyWhip.userID == -1 && PartyWhip.businessID == -1 && PartyWhip.error == 0;
+}
