dafny_verification/verify_login_signup.dfy
@@ -1,0 +1,125 @@
+class {:autocontracts} UserTable
+{
+    var id: int;
+    var username: string;
+    var password: string;
+    var email: string;
+
+      constructor(user: string, pass: string, email: string)
+      requires |user| > 0 && |pass| > 0 && |email| > 0;
+      ensures this.id == -1 && this.username == user && this.password == pass && this.email == email;
+      {
+          this.id := -1;
+          this.username := user;
+          this.password := pass;
+          this.email := email;
+      }
+      
+      method SetID(id: int)
+      requires id >= 0 && this.id == -1;
+      ensures this.id == id;
+      ensures this.username == old(this.username) && this.password == old(this.password) && this.email == old(this.email);
+      { this.id := id; }
+}
+
+method Login(UserDB: array<UserTable>, username: string, password: string) returns (userID: int)
+ensures UserDB[..] == old(UserDB[..]);
+ensures -1 <= userID < UserDB.Length;
+ensures userID == -1 ==> forall i:: 0 <= i < UserDB.Length ==> (UserDB[i].username != username || UserDB[i].password != password);
+ensures userID > -1 ==> UserDB[userID].username == username && UserDB[userID].password == password;
+{
+    var i := 0;
+    userID := -1;
+    while (i < UserDB.Length)
+    invariant 0 <= i <= UserDB.Length;
+    invariant userID == -1 ==> forall j:: 0 <= j < i ==> (UserDB[j].username != username || UserDB[j].password != password);
+    invariant userID > -1 ==> UserDB[userID].username == username && UserDB[userID].password == password;
+    {
+        if (UserDB[i].username == username && UserDB[i].password == password)
+        {
+            return i;
+        }
+        i := i + 1;
+    }
+}
+
+method SignUp(UserDB: array<UserTable>, newUser: UserTable) returns (err: bool)
+ensures UserDB[..] == old(UserDB[..]);
+ensures err ==> exists i:: 0 <= i < UserDB.Length && (UserDB[i].username == newUser.username || UserDB[i].email == newUser.email);
+ensures !err ==> forall i:: 0 <= i < UserDB.Length ==> (UserDB[i].username != newUser.username && UserDB[i].email != newUser.email);
+{
+    err := false;
+    var i := 0;
+    while (i < UserDB.Length && !err)
+    invariant 0 <= i <= UserDB.Length;
+    invariant err ==> exists j:: 0 <= j < i && (UserDB[j].username == newUser.username || UserDB[j].email == newUser.email);
+    invariant !err ==> forall j:: 0 <= j < i ==> (UserDB[j].username != newUser.username && UserDB[j].email != newUser.email);
+    {
+        if (UserDB[i].username == newUser.username)
+        {
+            err := true;
+        }
+        if (UserDB[i].email == newUser.email)
+        {
+            err := true;
+        }
+        i := i + 1;
+    }
+}
+
+method InsertUser(UserDB: array<UserTable>, newUser: UserTable, tempUsers: array<UserTable>) returns (newUserDB: array<UserTable>)
+modifies tempUsers;
+requires tempUsers.Length == UserDB.Length + 1;
+ensures newUserDB.Length == UserDB.Length + 1;
+ensures forall i:: 0 <= i < old(UserDB.Length) ==> newUserDB[i] == old(UserDB[i]);
+ensures newUserDB[old(UserDB.Length)] == newUser;
+{
+    forall i | 0 <= i < UserDB.Length { tempUsers[i] := UserDB[i]; }
+    tempUsers[UserDB.Length] := newUser;
+    return tempUsers;
+}
+
+method TestLoginSignup()
+{
+    var Users: array<UserTable> := new UserTable[0];
+    
+    var tmpUser := new UserTable("temp", "temp", "temp");
+    
+    /*
+      Testing success case: sign up new user and login
+    */
+    var admin := new UserTable("admin", "pass", "admin@admin.com");
+    assert admin.username == "admin" && admin.password == "pass" && admin.email == "admin@admin.com";
+    
+    var err_signup := SignUp(Users, admin);
+    assert !err_signup;
+    admin.SetID(Users.Length);
+    assert admin.username == "admin" && admin.password == "pass" && admin.email == "admin@admin.com" && admin.id == Users.Length;
+    
+    var tempUsers: array<UserTable> := new UserTable[Users.Length + 1][tmpUser];
+    Users := InsertUser(Users, admin, tempUsers);
+    assert Users.Length == 1 && Users[0] == admin;
+    
+    assert admin.username == "admin" && admin.password == "pass";
+    assert Users.Length == 1 && Users[0] == admin && Users[0].username == admin.username && Users[0].password == admin.password;
+    var err_login := Login(Users, "admin", "pass");
+    assert err_login == admin.id;
+    
+    /*
+      Testing error case: log in non-registered account
+    */
+    assert Users.Length == 1 && Users[0].username != "hacker";
+    err_login := Login(Users, "hacker", "hello, world");
+    assert err_login == -1;
+    
+    /*
+      Testing error case: sign up with used username
+    */
+    var bug := new UserTable("admin", "not_admin", "hello@world.com");
+    assert bug.username == "admin" && bug.password == "not_admin" && bug.email == "hello@world.com";
+    assert bug.username == admin.username && Users.Length == 1 && Users[0] == admin;
+    err_signup := SignUp(Users, bug);
+    assert err_signup;
+    err_signup := SignUp(Users, admin);
+    assert err_signup;
+}
